Adapt ExpandLetsCorrectness after rebase

pcuic/theories/PCUICExpandLetsCorrectness.v
@@ -12,7 +12,7 @@ From MetaCoq.PCUIC Require Import PCUICAst PCUICAstUtils PCUICOnOne PCUICCases P
      PCUICWeakeningEnvConv PCUICWeakeningEnvTyp 
      PCUICWeakeningConv PCUICWeakeningTyp PCUICClosedTyp
      PCUICReduction PCUICConversion PCUICCumulativity
-     PCUICUnivSubst PCUICGlobalEnv PCUICTyping PCUICGeneration
+     PCUICUnivSubst PCUICUnivSubstitutionTyp PCUICGlobalEnv PCUICTyping PCUICGeneration
      PCUICConversion PCUICOnFreeVars PCUICInductives
      PCUICValidity PCUICArities PCUICInversion PCUICInductiveInversion
      PCUICCases PCUICWellScopedCumulativity PCUICSpine PCUICSR
@@ -1417,7 +1417,7 @@ Require Import Morphisms.
 #[global] Instance map2_Proper {A B C} : Morphisms.Proper (pointwise_relation A (pointwise_relation B (@eq C)) ==> eq ==> eq ==> eq) map2.
 Proof.
   intros f g Hfg ? ? -> ? ? ->.
-  eapply PCUICNameless.map2_ext, Hfg.
+  eapply map2_ext, Hfg.
 Qed.
 
 Lemma map2_set_binder_name_eq nas Δ Δ' :
@@ -1515,9 +1515,9 @@ Lemma on_free_vars_ind_predicate_context {cf : checker_flags} {Σ : global_env_e
     (ind_predicate_context ind mdecl idecl).
 Proof.
   intros decli.
-  rewrite <- closedn_ctx_on_free_vars.
+  rewrite <- PCUICOnFreeVars.closedn_ctx_on_free_vars.
   eapply PCUICClosed.closed_ind_predicate_context; tea.
-  eapply (PCUICClosed.declared_minductive_closed (proj1 decli)).
+  eapply (PCUICClosedTyp.declared_minductive_closed (proj1 decli)).
 Qed.
 
 Lemma trans_case_predicate_context {cf} {Σ : PCUICEnvironment.global_env_ext}
@@ -1537,7 +1537,7 @@ Proof.
   rewrite /case_predicate_context /PCUICCases.case_predicate_context.
   rewrite /case_predicate_context_gen /PCUICCases.case_predicate_context_gen.
   rewrite /trans_local map_map2 map2_trans.
-  rewrite -PCUICUnivSubstitution.map2_map_r. f_equal.
+  rewrite -PCUICUnivSubstitutionConv.map2_map_r. f_equal.
   rewrite /p' /=. now rewrite forget_types_map_context.
   rewrite /pre_case_predicate_context_gen /inst_case_context.
   rewrite /PCUICCases.pre_case_predicate_context_gen /PCUICCases.inst_case_context.
@@ -1629,7 +1629,7 @@ Lemma on_free_vars_ctx_cstr_branch_context {cf} {Σ : global_env_ext} {wfΣ : wf
   on_free_vars_ctx (shiftnP (context_assumptions (ind_params mdecl)) xpred0) 
     (cstr_branch_context c.1 mdecl cdecl).
 Proof.
-  intros. eapply closedn_ctx_on_free_vars. eapply (PCUICInst.closedn_ctx_cstr_branch_context H).
+  intros. eapply closedn_ctx_on_free_vars. eapply (PCUICInstConv.closedn_ctx_cstr_branch_context H).
 Qed.
 
 Lemma typing_spine_wt {cf} {Σ : global_env_ext} {wfΣ : wf Σ} {args Γ x2 x3} :
@@ -1762,7 +1762,7 @@ Proof.
         etransitivity;tea. rewrite /expand_lets /expand_lets_k. simpl.
         rewrite -(length_of cum).
         rewrite -(red_context_rel_assumptions cum).
-        move: (PCUICSubstitution.context_assumptions_smash_context [] Γ0); cbn => <-. simpl.
+        move: (context_assumptions_smash_context [] Γ0); cbn => <-. simpl.
         change (Γ ,,, smash_context [] Γ0) with (Γ ,,, smash_context [] Γ0 ,,, []).
         eapply (untyped_substitution_equality_subst_conv (Γ' := [])); tea.
         now eapply red_terms_equality_terms in conv.
@@ -1775,7 +1775,7 @@ Proof.
         len => /=. rewrite -shiftnP_add. eapply on_free_vars_ctx_lift_context0.
         rewrite (red_context_rel_assumptions cum) addnP_shiftnP.
         now move/PCUICAlpha.is_closed_context_app_right: wfr.
-        rewrite PCUICSubstitution.context_assumptions_smash_context /=.
+        rewrite context_assumptions_smash_context /=.
         rewrite -[context_assumptions Γ0](smash_context_length []); cbn.
         relativize #|Γ0|.
         eapply is_open_term_lift.
@@ -1792,14 +1792,14 @@ Proof.
       rewrite /expand_lets /expand_lets_k. simpl.
       rewrite -(length_of cum).
       rewrite -(red_context_rel_assumptions cum).
-      move: (PCUICSubstitution.context_assumptions_smash_context [] Γ0); cbn => <-. simpl.
+      move: (context_assumptions_smash_context [] Γ0); cbn => <-. simpl.
       change (smash_context [] Γ0 ++ Γ) with (Γ ,,, smash_context [] Γ0 ,,, []).
       cbn. rewrite smash_context_acc /=.
       change (smash_context [] Γ0 ++ Γ) with (Γ ,,, smash_context [] Γ0 ,,, []).
       eapply (closed_red_red_subst (Γ := _ ,,, _) (Γ' := [])); tea.
       2:{ eapply PCUICContexts.untyped_subslet_extended_subst. }
       { now eapply weakening_is_closed_context. }
-      rewrite PCUICSubstitution.context_assumptions_smash_context /=.
+      rewrite context_assumptions_smash_context /=.
       rewrite -[context_assumptions Γ0](smash_context_length []); cbn.
       relativize #|Γ0|.
       eapply is_open_term_lift. 
@@ -2511,7 +2511,7 @@ Section wtcumul.
 
   Lemma cumul_decorate (Σ : global_env_ext) {wfΣ : wf Σ} Γ T U :
     isType Σ Γ T -> isType Σ Γ U ->
-    cumul Σ Γ T U ->
+    cumulAlgo Σ Γ T U ->
     wt_equality true Σ Γ T U.
   Proof.
     move/isType_wt => ht.
@@ -2529,7 +2529,7 @@ Section wtcumul.
 
   Lemma conv_decorate (Σ : global_env_ext) {wfΣ : wf Σ} Γ T U :
     wt Σ Γ T -> wt Σ Γ U ->
-    conv Σ Γ T U ->
+    convAlgo Σ Γ T U ->
     wt_equality false Σ Γ T U.
   Proof.
     intros ht hu.
@@ -2546,26 +2546,6 @@ Section wtcumul.
 
   Definition wt_equality_ctx {cf} le Σ := 
     All2_fold (fun Γ Γ' => All_decls_alpha_le le (fun le => wt_equality le Σ Γ)).
-    
-  Lemma cumul_ctx_decorate (Σ : global_env_ext) {wfΣ : wf Σ} Γ Δ :
-    wf_local Σ Γ ->
-    wf_local Σ Δ ->
-    cumul_context Σ Γ Δ ->
-    wt_equality_ctx true Σ Γ Δ.
-  Proof.
-    intros wfΓ wfΔ. induction 1. constructor; auto.
-    depelim wfΓ; depelim wfΔ; depelim p; constructor; auto. now apply IHX.
-    constructor; auto. apply cumul_decorate => //.
-    { destruct l0 as [s hs].
-      exists s. eapply context_cumulativity; tea. }
-    eapply IHX => //.
-    constructor; auto. apply conv_decorate => //.
-    { now exists t. }
-    { exists t0. eapply context_cumulativity; tea. }
-    eapply cumul_decorate => //.
-    destruct l1 as [s Hs]. exists s.
-    eapply context_cumulativity; tea.
-  Qed.
 
   Definition wt_equality_ctx_rel {cf} le Σ Γ := 
     All2_fold (fun Δ Δ' => All_decls_alpha_le le (fun le => wt_equality le Σ (Γ ,,, Δ))).
@@ -2575,7 +2555,7 @@ End wtcumul.
 Lemma trans_conv {cf} {Σ : PCUICEnvironment.global_env_ext} {Γ T U} {wfΣ : PCUICTyping.wf Σ} :
   wf_trans Σ ->
   wt_conv Σ Γ T U ->
-  conv (H := cf' cf) (trans_global Σ) (trans_local Γ) (trans T) (trans U).
+  convAlgo (H := cf' cf) (trans_global Σ) (trans_local Γ) (trans T) (trans U).
 Proof.
   intros wfΣ'; induction 1. 
   - constructor; auto.
@@ -2593,7 +2573,7 @@ Qed.
 Lemma trans_cumul {cf} {Σ : PCUICEnvironment.global_env_ext} {Γ T U} {wfΣ : PCUICTyping.wf Σ} :
   wf_trans Σ ->
   wt_cumul Σ Γ T U ->
-  cumul (H:=cf' cf) (trans_global Σ) (trans_local Γ) (trans T) (trans U).
+  cumulAlgo (H:=cf' cf) (trans_global Σ) (trans_local Γ) (trans T) (trans U).
 Proof.
   intros wfΣ'; induction 1. 
   - constructor; auto.
@@ -3735,7 +3715,7 @@ Proof.
       rewrite -trans_subst_instance_ctx.
       eapply weaken_ctx; eauto.
       clear hnth. eapply trans_declared_constructor in isdecl.
-      epose proof (typing_subst_instance_decl (trans_global Σ)
+      epose proof (PCUICUnivSubstitutionTyp.typing_subst_instance_decl (trans_global Σ)
         _ _ _ _ _ _ _ (proj1 (proj1 isdecl)) Hs).
       forward X2. now eapply trans_consistent_instance_ext.
       now rewrite trans_subst_instance_ctx trans_subst_instance.
@@ -3752,23 +3732,24 @@ Proof.
     eapply isType_mkApps_Ind_smash in hty as []; tea.
     erewrite <- (trans_case_predicate_context (Σ := Σ)); tea.
     2:{ eapply (wf_predicate_length_pars H0). }
-    eapply TT.type_Case; auto.
+    eapply TT.type_Case; auto. 4-5:split; auto.
     + now apply trans_declared_inductive.
-    + cbn. rewrite -trans_ind_predicate_context. eauto with pcuic. eauto with pcuic.
-      now eapply alpha_eq_trans.
+    + rewrite (trans_case_predicate_context (Σ := Σ) (Γ := Γ)); tea.
+      rewrite -trans_local_app. now eapply X3.
+    + rewrite trans_mkApps map_app in X8. now eapply X8.
     + now eapply trans_wf_predicate.
     + cbn. rewrite /id.
       now apply trans_consistent_instance_ext.
     + cbn [pparams pcontext].
       rewrite (trans_case_predicate_context (Σ := Σ) (Γ := Γ)); tea.
       now rewrite -trans_local_app. 
-    + rewrite (trans_case_predicate_context (Σ := Σ) (Γ := Γ)); tea.
-      rewrite -trans_local_app. now eapply X3.
+    + rewrite -trans_ind_predicate_context; eauto with pcuic.
+      now eapply alpha_eq_trans.
     + rewrite <- trans_global_ext_constraints.
       eassumption.
     + move: X5 X6. cbn.
       have wfctx : wf_local Σ (Γ ,,, (ind_params mdecl,,, ind_indices idecl)@[puinst p]).
-      { eapply PCUICWeakening.weaken_wf_local; tea. eapply on_minductive_wf_params_indices_inst; tea. }
+      { eapply PCUICWeakeningTyp.weaken_wf_local; tea. eapply on_minductive_wf_params_indices_inst; tea. }
       move: wfctx.
       clear -wfΣ X10.
       rewrite -map_app -[trans_local _ ++ _]trans_local_app.
@@ -3816,7 +3797,6 @@ Proof.
           eapply wf_local_closed_context in wfctx.
           now move: wfctx; rewrite on_free_vars_ctx_app /= => /andP[].
           exact X. }
-    + rewrite trans_mkApps map_app in X8. now eapply X8.
     + red. eapply Forall2_map_right, Forall2_map.
       eapply Forall2_All2 in H4.
       eapply All2i_All2_mix_left in X9; tea.
@@ -3935,14 +3915,14 @@ Proof.
       destruct a as [s Hs]. exists s; intuition eauto.
       solve_all. }
     eapply TT.type_Fix; auto.
+    + rewrite /trans_local map_app in X.
+      now eapply TT.All_local_env_app_inv in X as [].
     + now rewrite fix_guard_trans.
     + erewrite map_nth_error. 
       2: apply H0.
       destruct decl.
       unfold map_def.
       reflexivity.
-    + rewrite /trans_local map_app in X.
-      now eapply TT.All_local_env_app_inv in X as [].
     + eapply All_map, (All_impl X0).
       intuition auto. destruct X as [s [? ?]].
       exists s; intuition auto.
@@ -3964,14 +3944,14 @@ Proof.
       destruct a as [s Hs]. exists s; intuition eauto.
       solve_all. }
     eapply TT.type_CoFix; auto.
+    + rewrite /trans_local map_app in X.
+      now eapply TT.All_local_env_app_inv in X as [].
     + now eapply cofix_guard_trans.
-    + erewrite map_nth_error. 
+    + erewrite map_nth_error.
       2: eassumption.
       destruct decl.
       unfold map_def.
       reflexivity.
-    + rewrite /trans_local map_app in X.
-      now eapply TT.All_local_env_app_inv in X as [].
     + fold trans.
       eapply All_map, (All_impl X0).
       intros x [s ?]; exists s; intuition auto.
@@ -3988,7 +3968,9 @@ Proof.
   - eapply (type_equality (le:=true)).
     + eauto.
     + now exists s.
-    + eapply cumul_decorate in X4; tea.
+    + eapply cumulSpec_cumulAlgo_curry in X4; fvs.
+      eapply equality_forget in X4.
+      eapply cumul_decorate in X4; tea.
       2:eapply validity; tea.
       2:now exists s.
       eapply into_equality.
@@ -4647,32 +4629,115 @@ Proof.
   rewrite map_app. apply/in_or_app. firstorder.
 Qed.
 
+Lemma cumul_context_Spec_Algo {cf:checker_flags} {Σ} {wfΣ : wf Σ.1} {Γ Γ'} :
+  wf_local Σ Γ ->
+  wf_local Σ Γ' ->
+  PCUICCumulativitySpec.cumul_context Σ Γ' Γ ->
+  PCUICCumulativity.cumul_context Σ Γ' Γ.
+Proof.
+  intros wfΓ wfΓ'.
+  induction 1. constructor.
+  depelim wfΓ; depelim wfΓ'; depelim p; constructor; auto; constructor; auto.
+  - eapply cumulSpec_cumulAlgo_curry in c; tea. 2-4:fvs.
+    red in l. now eapply equality_forget in c.
+    rewrite (All2_fold_length X). fvs.
+  - eapply cumulSpec_cumulAlgo_curry in c0; tea. 2-4:fvs.
+    2:{ rewrite (All2_fold_length X). fvs. }
+    destruct l1; cbn in l0, l2.
+    eapply convSpec_convAlgo_curry in c; tea.
+    now apply equality_forget in c.
+    all:fvs. rewrite (All2_fold_length X). fvs.
+  - eapply cumulSpec_cumulAlgo_curry in c0; tea. 2-4:fvs.
+    2:{ rewrite (All2_fold_length X). fvs. }
+   now apply equality_forget in c0.
+Qed.
+
+Lemma context_cumulativity_spec {cf:checker_flags} {Σ} {wfΣ : wf Σ.1} Γ {t T Γ'} :
+  Σ ;;; Γ |- t : T ->
+  wf_local Σ Γ' ->
+  PCUICCumulativitySpec.cumul_context Σ Γ' Γ ->
+  Σ ;;; Γ' |- t : T.
+Proof.
+  intros h hΓ' e.
+  eapply PCUICContextConversionTyp.context_cumulativity; tea.
+  eapply cumul_context_Spec_Algo; tea. pcuic.
+Qed.
+(* 
+Lemma red_cumulSpec {cf:checker_flags} {Σ : global_env_ext} {Γ : context} {M N : term} :
+  red Σ Γ M N -> Σ ;;; Γ |- M =s N.
+Proof.
+  induction 1.
+  - now apply red1_cumulSpec.
+  - apply cumul_Refl.
+  -  *)
+
+Lemma trans_cumulSpec {cf} {Σ : PCUICEnvironment.global_env_ext} {Γ T U} {wfΣ : PCUICTyping.wf Σ} :
+  wf_trans Σ ->
+  isType Σ Γ T → isType Σ Γ U →
+  cumulSpec Σ Γ T U ->
+  cumulSpec (H:=cf' cf) (trans_global Σ) (trans_local Γ) (trans T) (trans U).
+Proof.
+  intros wfΣ' wtT wtU cum.
+  eapply cumulSpec_cumulAlgo_curry in cum; fvs.
+  eapply equality_forget in cum.
+  eapply cumul_decorate in cum; tea.
+  pose proof (trans_cumul wfΣ' cum); tea.
+  eapply (cumulAlgo_cumulSpec _ (le:=true)).
+  eapply into_equality; tea.
+  destruct wtT. apply trans_is_closed_context. fvs.
+  apply trans_on_free_vars; len; fvs.
+  apply trans_on_free_vars; len; fvs.
+  destruct wtT. fvs.
+Qed.
+
+Lemma trans_convSpec {cf} {Σ : PCUICEnvironment.global_env_ext} {Γ T U} {wfΣ : PCUICTyping.wf Σ} :
+  wf_trans Σ ->
+  wt Σ Γ T → wt Σ Γ U →
+  convSpec Σ Γ T U ->
+  convSpec (H:=cf' cf) (trans_global Σ) (trans_local Γ) (trans T) (trans U).
+Proof.
+  intros wfΣ' wtT wtU cum.
+  eapply convSpec_convAlgo_curry in cum; fvs.
+  eapply equality_forget in cum.
+  eapply conv_decorate in cum; tea.
+  pose proof (trans_conv wfΣ' cum); tea.
+  eapply (cumulAlgo_cumulSpec _ (le:=false)).
+  destruct wtT, wtU.
+  eapply into_equality; tea.
+  apply trans_is_closed_context. fvs.
+  apply trans_on_free_vars; len; fvs.
+  apply trans_on_free_vars; len; fvs.
+  1-2:destruct wtT; fvs.
+  destruct wtU. fvs.
+Qed.
+
 Lemma trans_cumul_ctx_rel {cf} {Σ : global_env_ext} {wfΣ : wf Σ} {Γ Δ Δ'} :
   wf_trans Σ ->
   wf_local Σ (Γ ,,, Δ) ->
   wf_local Σ (Γ ,,, Δ') ->
-  PCUICConversion.cumul_ctx_rel Σ Γ Δ Δ' ->
-  PCUICConversion.cumul_ctx_rel (cf:=cf' cf) (trans_global Σ) (trans_local Γ) (trans_local Δ) (trans_local Δ').
+  cumul_ctx_rel Σ Γ Δ Δ' ->
+  cumul_ctx_rel (cf:=cf' cf) (trans_global Σ) (trans_local Γ) (trans_local Δ) (trans_local Δ').
 Proof.
   intros wf' wfl wfr.
   induction 1; cbn; constructor; auto.
   eapply IHX. now depelim wfl. now depelim wfr.
   destruct p; constructor; cbn in *; auto.
-  - rewrite -trans_local_app. eapply (trans_cumul (Σ := Σ)) => //.
+  - rewrite -trans_local_app. 
     depelim wfl; depelim wfr. red in l, l0.
-    eapply cumul_decorate; tea. 
-    { destruct l0 as [s Hs]. exists s. eapply context_cumulativity; tea.
+    destruct l0 as [s Hs]. destruct l as [s' Hs'].
+    eapply trans_cumulSpec in c; tea.
+    { now exists s'. }
+    { exists s. eapply context_cumulativity_spec; tea.
       eapply All2_fold_app. reflexivity. apply X. }
-  - rewrite -trans_local_app. eapply (trans_conv (Σ := Σ)) => //.
-    depelim wfl; depelim wfr. red in l, l0.
-    eapply conv_decorate; tea. auto.
+  - rewrite -trans_local_app. depelim wfl; depelim wfr. red in l, l0.
+    eapply (trans_convSpec (Σ := Σ)) => //.
     now exists T. 
-    { red in l2. exists T'. eapply context_cumulativity; tea.
+    { red in l2. exists T'. eapply context_cumulativity_spec; tea.
       eapply All2_fold_app. reflexivity. apply X. }
-  - rewrite -trans_local_app. eapply (trans_cumul (Σ := Σ)) => //.
+  - rewrite -trans_local_app.
     depelim wfl; depelim wfr. red in l, l0.
-    eapply cumul_decorate; tea. 
-    { destruct l1 as [s Hs]. exists s. eapply context_cumulativity; tea.
+    eapply (trans_cumulSpec (Σ := Σ)) => //.
+    { destruct l1 as [s Hs]. exists s. eapply context_cumulativity_spec; tea.
       eapply All2_fold_app. reflexivity. apply X. }
 Qed.
 
@@ -4695,8 +4760,8 @@ Lemma cumul_type_irrelevance {cf} {Σ : global_env_ext} {wfΣ : wf Σ} {Γ Γ' T
   #|Γ| = #|Γ'| ->
   assumption_context Γ ->
   assumption_context Γ' ->
-  cumul Σ Γ T U ->
-  cumul Σ Γ' T U.
+  cumulAlgo Σ Γ T U ->
+  cumulAlgo Σ Γ' T U.
 Proof.
   intros wf len ass ass'.
   induction 1. constructor; auto.
@@ -4713,11 +4778,19 @@ Section wtcumul'.
   Reserved Notation " Σ ;;; Γ | Γ' |-- t <=[ le ] u " (at level 50, Γ, Γ' , le, t, u at next level).
 
   Inductive wt_equality_hetero (le : bool) (Σ : global_env_ext) (Γ Γ' : context) : term -> term -> Type :=
-  | wt_cumul_refl' t u : compare_term le Σ.1 (global_ext_constraints Σ) t u -> Σ ;;; Γ | Γ' |-- t <=[le] u 
+  | wt_cumul_refl' t u : wt Σ Γ t -> wt Σ Γ' u ->
+    compare_term le Σ.1 (global_ext_constraints Σ) t u -> Σ ;;; Γ | Γ' |-- t <=[le] u 
   | wt_cumul_red_l' t u v : wt_red1 Σ Γ t v -> Σ ;;; Γ | Γ' |-- v <=[le] u -> Σ ;;; Γ | Γ' |-- t <=[le] u
   | wt_cumul_red_r' t u v : Σ ;;; Γ | Γ' |-- t <=[le] v -> wt_red1 Σ Γ' u v -> Σ ;;; Γ | Γ' |-- t <=[le] u
   where " Σ ;;; Γ | Γ' |-- t <=[ le ] u " := (wt_equality_hetero le Σ Γ Γ' t u) : type_scope.
     
+  Lemma wt_equality_hetero_inv {le Σ Γ Γ' T U} : 
+    wt_equality_hetero le Σ Γ Γ' T U ->
+    wt Σ Γ T × wt Σ Γ' U.
+  Proof.
+    induction 1; intuition auto. destruct w; auto. destruct w; auto.
+  Qed.
+
   Definition wt_cumul_hetero := wt_equality_hetero true.
   Definition wt_conv_hetero := wt_equality_hetero false.
 
@@ -4726,14 +4799,14 @@ Section wtcumul'.
     #|Γ| = #|Γ'| ->
     assumption_context Γ ->
     assumption_context Γ' ->  
-    cumul Σ Γ T U ->
+    cumulAlgo Σ Γ T U ->
     wt_equality_hetero true Σ Γ Γ' T U.
   Proof.
     move/isType_wt => ht.
     move/isType_wt => hu.
     move=> hlen ass ass'.
     induction 1. 
-    - constructor. auto.
+    - constructor; auto.
     - pose proof (wt_red ht r).
       econstructor 2.
       econstructor; tea.
@@ -4745,22 +4818,33 @@ Section wtcumul'.
       econstructor; tea.
   Qed.
 
+  Lemma wt_convSpec_convAlgo {Σ : global_env_ext} {wfΣ : wf Σ} {Γ Γ' T U} :
+    wt Σ Γ T -> wt Σ Γ' U ->
+    #|Γ| = #|Γ'| ->
+    convSpec Σ Γ T U ->
+    convAlgo Σ Γ T U.
+  Proof.
+    intros [] [] len c.
+    eapply convSpec_convAlgo_curry in c; tea.
+    now eapply equality_forget in c. fvs. fvs. rewrite len; fvs.
+  Qed.
 
   Lemma conv_decorate_hetero (Σ : global_env_ext) {wfΣ : wf Σ} {Γ Γ' T U} :
     wt Σ Γ T -> wt Σ Γ' U ->
     #|Γ| = #|Γ'| ->
     assumption_context Γ ->
     assumption_context Γ' ->  
-    conv Σ Γ T U ->
+    convSpec Σ Γ T U ->
     wt_equality_hetero false Σ Γ Γ' T U.
   Proof.
-    move=> ht hu hlen ass ass'.
-    induction 1. 
-    - constructor. auto.
+    move=> ht hu hlen ass ass' c.
+    eapply wt_convSpec_convAlgo in c; tea.
+    induction c. 
+    - constructor; auto.
     - pose proof (wt_red ht r).
       econstructor 2.
       econstructor; tea.
-      eapply IHX; tea.
+      eapply IHc; tea.
     - eapply context_pres_let_bodies_red1 in r.
       2:eapply pres_let_bodies_assumption_context; tea.
       pose proof (wt_red hu r).
@@ -4784,7 +4868,7 @@ Lemma trans_cumul' {cf} {Σ : PCUICEnvironment.global_env_ext} {Γ Γ' T U} {wf�
   #|Γ| = #|Γ'| ->
   assumption_context Γ ->
   assumption_context Γ' ->  
-  cumul (H:=cf' cf) (trans_global Σ) (trans_local Γ) (trans T) (trans U).
+  cumulAlgo (H:=cf' cf) (trans_global Σ) (trans_local Γ) (trans T) (trans U).
 Proof.
   intros wfΣ'; induction 1. 
   - constructor; auto.
@@ -4810,7 +4894,7 @@ Lemma trans_conv' {cf} {Σ : PCUICEnvironment.global_env_ext} {Γ Γ' T U} {wfΣ
   #|Γ| = #|Γ'| ->
   assumption_context Γ ->
   assumption_context Γ' ->  
-  conv (H:=cf' cf) (trans_global Σ) (trans_local Γ) (trans T) (trans U).
+  convAlgo (H:=cf' cf) (trans_global Σ) (trans_local Γ) (trans T) (trans U).
 Proof.
   intros wfΣ'; induction 1. 
   - constructor; auto.
@@ -4830,6 +4914,22 @@ Proof.
     eapply pres_let_bodies_assumption_context; tea. now symmetry. 
 Qed.
 
+Lemma trans_convSpec' {cf} {Σ : PCUICEnvironment.global_env_ext} {Γ Γ' T U} {wfΣ : PCUICTyping.wf Σ} :
+  wf_trans Σ ->
+  wt_conv_hetero Σ Γ Γ' T U ->
+  #|Γ| = #|Γ'| ->
+  assumption_context Γ ->
+  assumption_context Γ' ->  
+  convSpec (H:=cf' cf) (trans_global Σ) (trans_local Γ) (trans T) (trans U).
+Proof.
+  intros wfΣ' cv len ass ass'.
+  eapply (cumulAlgo_cumulSpec _ (le:=false)).
+  eapply into_equality; [eapply trans_conv'; tea|eapply wt_equality_hetero_inv in cv as [[] []]..].
+  eapply trans_is_closed_context; fvs.
+  eapply trans_on_free_vars; rewrite map_length; fvs.
+  eapply trans_on_free_vars; rewrite map_length len; fvs.
+Qed.
+
 Lemma trans_cumul_ctx_rel' {cf} {Σ : global_env_ext} {wfΣ : wf Σ} {Γ Γ' Δ Δ'} :
   wf_trans Σ ->
   wf_local Σ (Γ ,,, Δ) ->
@@ -4837,20 +4937,31 @@ Lemma trans_cumul_ctx_rel' {cf} {Σ : global_env_ext} {wfΣ : wf Σ} {Γ Γ' Δ 
   #|Γ| = #|Γ'| ->
   assumption_context (Γ ,,, Δ) ->
   assumption_context (Γ' ,,, Δ') ->
-  PCUICConversion.cumul_ctx_rel Σ Γ Δ Δ' ->
-  PCUICConversion.cumul_ctx_rel (cf:=cf' cf) (trans_global Σ) (trans_local Γ) (trans_local Δ) (trans_local Δ').
+  cumul_ctx_rel Σ Γ Δ Δ' ->
+  cumul_ctx_rel (cf:=cf' cf) (trans_global Σ) (trans_local Γ) (trans_local Δ) (trans_local Δ').
 Proof.
   intros wf' wfl wfr eqlen ass ass'.
   induction 1; cbn; constructor; auto.
   eapply IHX. now depelim wfl. now depelim wfr. now depelim ass. now depelim ass'.
   destruct p; constructor; cbn in *; auto.
-  - rewrite -trans_local_app. eapply (trans_cumul' (Σ := Σ) (Γ' := Γ' ,,, Γ'0)) => //.
-    depelim wfl; depelim wfr. red in l, l0.
-    eapply cumul_decorate_hetero; tea.
+  - rewrite -trans_local_app.
+    depelim wfl; depelim wfr. red in l, l0. destruct l, l0.
+    eapply (cumulAlgo_cumulSpec _ (le:=true)).
+    apply into_equality.
+    eapply (trans_cumul' (Σ := Σ) (Γ' := Γ' ,,, Γ'0)) => //.
+    eapply cumul_decorate_hetero; tea. now eexists. now eexists.
     len. now rewrite (All2_fold_length X) eqlen.
     now depelim ass. now depelim ass'.
-    len. now rewrite (All2_fold_length X) eqlen.
+    eapply cumulSpec_cumulAlgo_curry in c; eauto.
+    now apply equality_forget in c. fvs. eapply (subject_is_open_term t).
+    len.
+    rewrite (All2_fold_length X) eqlen.
+    rewrite -app_length; fvs. len. eapply All2_fold_length in X. lia.
     now depelim ass. now depelim ass'.
+    eapply trans_is_closed_context; fvs.
+    eapply trans_on_free_vars; rewrite map_length /app_context; fvs.
+    eapply trans_on_free_vars; len.
+    rewrite (All2_fold_length X) eqlen -app_length; fvs.
   - elimtype False. depelim ass.
   - elimtype False; depelim ass.
 Qed.
@@ -4934,7 +5045,7 @@ Lemma wt_subst_instance {cf} {Σ : global_env} {ϕ : universes_decl} {Γ T u uni
   wt (Σ, ϕ) Γ@[u] T@[u].
 Proof.
   intros wf [s Hs] cu. exists (s@[u]).
-  eapply typing_subst_instance'; tea.
+  eapply PCUICUnivSubstitutionTyp.typing_subst_instance'; tea.
   eapply sub_context_set_empty.
 Qed.
 
@@ -5152,7 +5263,7 @@ Proof.
             destruct onArity as [s Hs].
             rewrite -it_mkProd_or_LetIn_app in Hs.
             eapply type_it_mkProd_or_LetIn_inv in Hs as [? [? [Hs _]]].
-            eapply sorts_local_ctx_All_local_env in Hs; eauto. 
+            eapply PCUICClosedConv.sorts_local_ctx_All_local_env in Hs; eauto. 
             now rewrite app_context_nil_l in Hs. }
           { eapply wf_local_smash_end. 
             eapply sorts_local_ctx_wf_local in on_cargs => //.
@@ -5272,7 +5383,7 @@ Proof.
               rewrite -shiftnP_add.
               rewrite (on_free_vars_expand_lets_k _ _ 0) //  shiftnP_add // /= shiftnP_add //. }
             rewrite -!trans_subst_instance.
-            eapply (trans_conv' (Σ := (Σ0, univs')) 
+            eapply (trans_convSpec' (Σ := (Σ0, univs')) 
               (Γ' := (arities_context (ind_bodies m),,,
               SE.smash_context []
                 (ind_params m,,, SE.smash_context [] (cstr_args cdecl)))@[u'])); eauto.
